extraction/ExtractKuiper.fst
@@ -288,72 +288,107 @@ let hta (e : mlexpr) : option (string & list mlty & list mlexpr) =
 
 (* Substitutes the variable [v] in the expression [e] with the expression [e'].
    i.e e[v := e']. *)
-let rec ml_subst (e : mlexpr) (v : mlident) (e' : mlexpr) : mlexpr =
-  match e.expr with
-  | MLE_Const _ -> e
-  | MLE_Var v' -> if v = v' then e' else e
-  | MLE_Name _ -> e
-  | MLE_Let ((flavor, lbs), e2) ->
-    let lbs' = lbs |> List.map (fun lb -> {lb with mllb_def = ml_subst lb.mllb_def v e'}) in
-    let e2' = ml_subst e2 v e' in
-    { e with expr = MLE_Let ((flavor, lbs'), e2') }
-  | MLE_App (head, args) ->
-    let head' = ml_subst head v e' in
-    let args' = List.map (fun arg -> ml_subst arg v e') args in
-    { e with expr = MLE_App (head', args') }
-  | MLE_TApp (head, args) ->
-    let head' = ml_subst head v e' in
-    { e with expr = MLE_TApp (head', args) }
-  | MLE_Fun (bs, e2) ->
-    (* fully named, no clashses should occur. *)
-    let e2' = ml_subst e2 v e' in
-    { e with expr = MLE_Fun (bs, e2') }
-  | MLE_Match (e1, branches) ->
-    let e1' = ml_subst e1 v e' in
-    let branches' =
-      branches |> List.map (fun (p, e2, e3) ->
-        let e2' = BU.map_opt e2 (fun e2 -> ml_subst e2 v e') in
-        let e3' = ml_subst e3 v e' in
-        (p, e2', e3')
-      )
-    in
-    { e with expr = MLE_Match (e1', branches') }
-  | MLE_Coerce (e1, t1, t2) ->
-    let e1' = ml_subst e1 v e' in
-    { e with expr = MLE_Coerce (e1', t1, t2) }
-  | MLE_Seq es ->
-    let es' = List.map (fun e -> ml_subst e v e') es in
-    { e with expr = MLE_Seq es' }
-  | MLE_Tuple es ->
-    let es' = List.map (fun e -> ml_subst e v e') es in
-    { e with expr = MLE_Tuple es' }
-  | MLE_Record (p, t, fields) ->
-    let fields' = List.map (fun (f, e) -> f, ml_subst e v e') fields in
-    { e with expr = MLE_Record (p, t, fields') }
-  | MLE_Proj (e1, f) ->
-    let e1' = ml_subst e1 v e' in
-    { e with expr = MLE_Proj (e1', f) }
-  | MLE_If (e1, e2, e3) ->
-    let e1' = ml_subst e1 v e' in
-    let e2' = ml_subst e2 v e' in
-    let e3' = BU.map_opt e3 (fun e3 -> ml_subst e3 v e') in
-    { e with expr = MLE_If (e1', e2', e3') }
-  | MLE_Raise (p, args) ->
-    let args' = List.map (fun arg -> ml_subst arg v e') args in
-    { e with expr = MLE_Raise (p, args') }
-  | MLE_Try (e1, branches) ->
-    let e1' = ml_subst e1 v e' in
-    let branches' =
-      branches |> List.map (fun (p, e2, e3) ->
-        let e2' = BU.map_opt e2 (fun e2 -> ml_subst e2 v e') in
-        let e3' = ml_subst e3 v e' in
-        (p, e2', e3')
-      )
-    in
-    { e with expr = MLE_Try (e1', branches') }
-  | MLE_CTor (p, args) ->
-    let args' = List.map (fun arg -> ml_subst arg v e') args in
-    { e with expr = MLE_CTor (p, args') }
+let rec ml_visit (pre post : mlexpr -> mlexpr) (e : mlexpr) : mlexpr =
+  let e = pre e in
+  let e =
+    match e.expr with
+    | MLE_Const _ -> e
+    | MLE_Var _ -> e
+    | MLE_Name _ -> e
+    | MLE_Let ((flavor, lbs), e2) ->
+      let lbs' = lbs |> List.map (fun lb -> {lb with mllb_def = ml_visit pre post lb.mllb_def}) in
+      let e2' = ml_visit pre post e2 in
+      { e with expr = MLE_Let ((flavor, lbs'), e2') }
+    | MLE_App (head, args) ->
+      let head' = ml_visit pre post head in
+      let args' = List.map (fun arg -> ml_visit pre post arg) args in
+      { e with expr = MLE_App (head', args') }
+    | MLE_TApp (head, tyargs) ->
+      let head' = ml_visit pre post head in
+      { e with expr = MLE_TApp (head', tyargs) }
+    | MLE_Fun (bs, e2) ->
+      (* fully named, no clashses should occur. *)
+      let e2' = ml_visit pre post e2 in
+      { e with expr = MLE_Fun (bs, e2') }
+    | MLE_Match (e1, branches) ->
+      let e1' = ml_visit pre post e1 in
+      let branches' =
+        branches |> List.map (fun (p, e2, e3) ->
+          let e2' = BU.map_opt e2 (fun e2 -> ml_visit pre post e2) in
+          let e3' = ml_visit pre post e3 in
+          (p, e2', e3')
+        )
+      in
+      { e with expr = MLE_Match (e1', branches') }
+    | MLE_Coerce (e1, t1, t2) ->
+      let e1' = ml_visit pre post e1 in
+      { e with expr = MLE_Coerce (e1', t1, t2) }
+    | MLE_Seq es ->
+      let es' = List.map (fun e -> ml_visit pre post e) es in
+      { e with expr = MLE_Seq es' }
+    | MLE_Tuple es ->
+      let es' = List.map (fun e -> ml_visit pre post e) es in
+      { e with expr = MLE_Tuple es' }
+    | MLE_Record (p, t, fields) ->
+      let fields' = List.map (fun (f, e) -> f, ml_visit pre post e) fields in
+      { e with expr = MLE_Record (p, t, fields') }
+    | MLE_Proj (e1, f) ->
+      let e1' = ml_visit pre post e1 in
+      { e with expr = MLE_Proj (e1', f) }
+    | MLE_If (e1, e2, e3) ->
+      let e1' = ml_visit pre post e1 in
+      let e2' = ml_visit pre post e2 in
+      let e3' = BU.map_opt e3 (fun e3 -> ml_visit pre post e3) in
+      { e with expr = MLE_If (e1', e2', e3') }
+    | MLE_Raise (p, args) ->
+      let args' = List.map (fun arg -> ml_visit pre post arg) args in
+      { e with expr = MLE_Raise (p, args') }
+    | MLE_Try (e1, branches) ->
+      let e1' = ml_visit pre post e1 in
+      let branches' =
+        branches |> List.map (fun (p, e2, e3) ->
+          let e2' = BU.map_opt e2 (fun e2 -> ml_visit pre post e2) in
+          let e3' = ml_visit pre post e3 in
+          (p, e2', e3')
+        )
+      in
+      { e with expr = MLE_Try (e1', branches') }
+    | MLE_CTor (p, args) ->
+      let args' = List.map (fun arg -> ml_visit pre post arg) args in
+      { e with expr = MLE_CTor (p, args') }
+  in
+  post e
+
+(* Substitutes the variable [v] in the expression [e] with the expression [e'].
+   i.e e[v := e']. *)
+let ml_subst (e : mlexpr) (v : mlident) (e' : mlexpr) : mlexpr =
+  let subst1 (e : mlexpr) : mlexpr =
+    match e.expr with
+    | MLE_Var v' when v = v' -> e'
+    | _ -> e
+  in
+  ml_visit subst1 id e
+
+let collapse_tuple_proj (e : mlexpr) : mlexpr =
+  let subst1 (e0 : mlexpr) : mlexpr =
+    match e0.expr with
+    | MLE_App ({ expr = MLE_TApp ({ expr = MLE_Name f }, _) }, [e]) when string_of_mlpath f = "FStar.Pervasives.Native.fst" -> (
+      let e = unmagic e in
+      match e.expr with
+      | MLE_Tuple [x;y] ->
+        x
+      | _ -> e0
+    )
+    | MLE_App ({ expr = MLE_TApp ({ expr = MLE_Name f }, _) }, [e]) when string_of_mlpath f = "FStar.Pervasives.Native.snd" -> (
+      let e = unmagic e in
+      match e.expr with
+      | MLE_Tuple [x;y] ->
+        y
+      | _ -> e0
+    )
+    | _ -> e0
+  in
+  ml_visit id subst1 e
 
 let is_lid (s:string) (e : mlexpr) : bool =
   match e.expr with
@@ -423,7 +458,7 @@ let extract_kcall (env : Krml.env) (kdesc : mlexpr) : option mlexpr =
       let mk_c_sh (desc : list (mlexpr & mlexpr)) : mlexpr & mlexpr =
         let rec aux (off : mlexpr) (desc : list (mlexpr & mlexpr)) : mlexpr & mlexpr =
           match desc with
-          | [] -> ml_unit, off
+          | [] -> intlit 123, off
           | (e_sz, len) :: desc' ->
             let off' = sizet_add off (sizet_mul e_sz len) in
             // let this_one =
@@ -501,6 +536,7 @@ let extract_kcall (env : Krml.env) (kdesc : mlexpr) : option mlexpr =
       let kf = apply_lam kf ml_blockidx in
       let kf = apply_lam kf ml_threadidx in
       let kf = apply_lam kf ml_unit in
+      let kf = collapse_tuple_proj kf in
       let kf = hoist env kf in
       let hd, rest_args = head_and_args kf in
       if Nil? rest_args then // is this really a problem?
